Weidenbach_Book/Watched_Literals_Watch_List_Domain.thy
@@ -1,11 +1,11 @@
 theory Watched_Literals_Watch_List_Domain
-  imports Watched_Literals_Watch_List
-    Array_UInt
+  imports Watched_Literals_Watch_List Array_UInt
 begin
 
 text \<open>We refine the implementation by adding a \<^emph>\<open>domain\<close> on the literals\<close>
 
 no_notation Ref.update ("_ := _" 62)
+
 
 subsection \<open>State Conversion\<close>
 
@@ -19,19 +19,19 @@ type_synonym clause_wl = \<open>uint32 array\<close>
 type_synonym unit_lits_wl = \<open>uint32 list list\<close>
 
 
-
 subsection \<open>Refinement\<close>
 
+subsubsection \<open>Set of all literals of the problem\<close>
 
-definition all_lits :: \<open>_ \<Rightarrow> _ \<Rightarrow> 'v literal multiset\<close> where
-  \<open>all_lits S NUE \<equiv> all_lits_of_mm ((\<lambda>C. mset (fst C)) `# ran_m S
-        + NUE)\<close>
+definition all_lits :: \<open>('a, 'v literal list \<times> 'b) fmap \<Rightarrow> 'v literal multiset multiset \<Rightarrow>
+   'v literal multiset\<close> where
+  \<open>all_lits S NUE = all_lits_of_mm ((\<lambda>C. mset (fst C)) `# ran_m S + NUE)\<close>
 
 abbreviation all_lits_st :: \<open>'v twl_st_wl \<Rightarrow> 'v literal multiset\<close> where
   \<open>all_lits_st S \<equiv> all_lits (get_clauses_wl S) (get_unit_clauses_wl S)\<close>
 	
 definition all_atms :: \<open>_ \<Rightarrow> _ \<Rightarrow> 'v multiset\<close> where
-  \<open>all_atms N NUE \<equiv> atm_of `# all_lits N NUE\<close>
+  \<open>all_atms N NUE = atm_of `# all_lits N NUE\<close>
 
 abbreviation all_atms_st :: \<open>'v twl_st_wl \<Rightarrow> 'v multiset\<close> where
   \<open>all_atms_st S \<equiv> atm_of `# all_lits_st S\<close>
@@ -113,6 +113,7 @@ end
 definition blits_in_\<L>\<^sub>i\<^sub>n :: \<open>nat twl_st_wl \<Rightarrow> bool\<close> where
   \<open>blits_in_\<L>\<^sub>i\<^sub>n S \<longleftrightarrow>
     (\<forall>L \<in># \<L>\<^sub>a\<^sub>l\<^sub>l (all_atms_st S). \<forall>(i, K, b) \<in> set (watched_by S L). K \<in># \<L>\<^sub>a\<^sub>l\<^sub>l (all_atms_st S))\<close>
+
 
 definition literals_are_\<L>\<^sub>i\<^sub>n :: \<open>nat multiset \<Rightarrow> nat twl_st_wl \<Rightarrow> bool\<close> where
   \<open>literals_are_\<L>\<^sub>i\<^sub>n \<A> S \<equiv> (is_\<L>\<^sub>a\<^sub>l\<^sub>l \<A> (all_lits_st S) \<and> blits_in_\<L>\<^sub>i\<^sub>n S)\<close>
@@ -573,6 +574,9 @@ lemma literals_are_\<L>\<^sub>i\<^sub>n_all_atms_stD[dest]:
   unfolding literals_are_\<L>\<^sub>i\<^sub>n_def
   by auto
 
+lemma blits_in_\<L>\<^sub>i\<^sub>n_set_conflict[simp]: \<open>blits_in_\<L>\<^sub>i\<^sub>n (set_conflict_wl D S) = blits_in_\<L>\<^sub>i\<^sub>n S\<close>
+  by (cases S) (auto simp: blits_in_\<L>\<^sub>i\<^sub>n_def set_conflict_wl_def)
+
 lemma unit_propagation_inner_loop_body_wl_D_spec:
   fixes S :: \<open>nat twl_st_wl\<close> and K :: \<open>nat literal\<close> and w :: nat
   assumes
@@ -659,8 +663,7 @@ proof -
     by (cases S; cases \<open>j=w\<close>) (auto simp: keep_watch_def)
   have update_blit_wl: \<open>update_blit_wl K x1a b' j w
         (get_clauses_wl (keep_watch K j w S) \<propto> x1a !
-          (1 -
-          (if get_clauses_wl (keep_watch K j w S) \<propto> x1a ! 0 = K then 0 else 1)))
+          (1 - (if get_clauses_wl (keep_watch K j w S) \<propto> x1a ! 0 = K then 0 else 1)))
         (keep_watch K j w S)
         \<le> \<Down> {((j', n', T'), j, n, T).
             j' = j \<and> n' = n \<and> T = T' \<and> literals_are_\<L>\<^sub>i\<^sub>n \<A> T'}
@@ -753,7 +756,7 @@ proof -
     have [simp]: \<open>blits_in_\<L>\<^sub>i\<^sub>n
         (set_conflict_wl D (a, b, c, d, e, fb, g(K := g K[j := de]))) \<longleftrightarrow>
         blits_in_\<L>\<^sub>i\<^sub>n ((a, b, c, d, e, fb, g(K := g K[j := de])))\<close>
-      for a b c d e f fb g de D
+      for a b c d e f g de D
       by (auto simp: blits_in_\<L>\<^sub>i\<^sub>n_def set_conflict_wl_def)
 
     have [simp]: \<open>x1a = x1\<close>
@@ -768,7 +771,7 @@ proof -
           dest!: multi_member_split split: if_splits)
     then show ?thesis
       using assms that by (cases S) (auto simp: keep_watch_def literals_are_\<L>\<^sub>i\<^sub>n_set_conflict_wl
-          literals_are_\<L>\<^sub>i\<^sub>n_def blits_in_\<L>\<^sub>i\<^sub>n_keep_watch')
+        literals_are_\<L>\<^sub>i\<^sub>n_def blits_in_\<L>\<^sub>i\<^sub>n_keep_watch')
   qed
   have bin_set_conflict:
     \<open>((j + 1, w + 1, set_conflict_wl (get_clauses_wl (keep_watch K j w S) \<propto> x1b) (keep_watch K j w S)), j + 1, w + 1,
@@ -818,15 +821,14 @@ proof -
       \<open>polarity (get_trail_wl (keep_watch K j w S)) x1a \<noteq> Some False\<close> and
       \<open>propagate_proper_bin_case K x1a (keep_watch K j w S) x1\<close>
     for x1 x2 x1a x2a x1b x2b x1c x2c
-  unfolding propagate_lit_wl_def S
+  unfolding propagate_lit_wl_def S propagate_proper_bin_case_def
   apply clarify
   apply refine_vcg
   using that \<A>\<^sub>i\<^sub>n
-  by (auto simp: clauses_def unit_prop_body_wl_find_unwatched_inv_def
-        propagate_proper_bin_case_def
-        mset_take_mset_drop_mset' S unit_prop_body_wl_D_inv_def unit_prop_body_wl_inv_def
-        ran_m_mapsto_upd unit_propagation_inner_loop_body_l_inv_def blits_in_\<L>\<^sub>i\<^sub>n_propagate
-        state_wl_l_def image_mset_remove1_mset_if literals_are_\<L>\<^sub>i\<^sub>n_def)
+  by (simp_all add: unit_prop_body_wl_find_unwatched_inv_def
+        propagate_proper_bin_case_def unit_prop_body_wl_inv_def
+        S unit_prop_body_wl_D_inv_def keep_watch_def state_wl_l_def literals_are_\<L>\<^sub>i\<^sub>n_def
+	Let_def blits_in_\<L>\<^sub>i\<^sub>n_propagate)
   show ?thesis
     unfolding unit_propagation_inner_loop_body_wl_D_def find_unwatched_wl_def[symmetric]
     unfolding unit_propagation_inner_loop_body_wl_def
@@ -876,8 +878,7 @@ proof -
 qed
 
 
-lemma
-  shows unit_propagation_inner_loop_body_wl_D_unit_propagation_inner_loop_body_wl_D:
+lemma unit_propagation_inner_loop_body_wl_D_unit_propagation_inner_loop_body_wl_D:
   \<open>(uncurry3 unit_propagation_inner_loop_body_wl_D, uncurry3 unit_propagation_inner_loop_body_wl) \<in>
     [\<lambda>(((K, j), w), S). literals_are_\<L>\<^sub>i\<^sub>n \<A> S \<and> K \<in># \<L>\<^sub>a\<^sub>l\<^sub>l \<A>]\<^sub>f
     Id \<times>\<^sub>r Id \<times>\<^sub>r Id \<times>\<^sub>r Id \<rightarrow> \<langle>nat_rel \<times>\<^sub>r nat_rel \<times>\<^sub>r
@@ -903,11 +904,11 @@ proof -
     by fastforce+
 qed
 
-definition (in isasat_input_ops) unit_propagation_inner_loop_wl_loop_D
+definition unit_propagation_inner_loop_wl_loop_D
   :: \<open>nat literal \<Rightarrow> nat twl_st_wl \<Rightarrow> (nat \<times> nat \<times> nat twl_st_wl) nres\<close>
 where
   \<open>unit_propagation_inner_loop_wl_loop_D L S\<^sub>0 = do {
-    ASSERT(L \<in># \<L>\<^sub>a\<^sub>l\<^sub>l);
+    ASSERT(L \<in># \<L>\<^sub>a\<^sub>l\<^sub>l (all_atms_st S\<^sub>0));
     let n = length (watched_by S\<^sub>0 L);
     WHILE\<^sub>T\<^bsup>unit_propagation_inner_loop_wl_loop_D_inv L\<^esup>
       (\<lambda>(j, w, S). w < n \<and> get_conflict_wl S = None)
@@ -919,27 +920,29 @@ where
   \<close>
 
 lemma unit_propagation_inner_loop_wl_spec:
-  assumes \<A>\<^sub>i\<^sub>n: \<open>literals_are_\<L>\<^sub>i\<^sub>n S\<close> and K: \<open>K \<in># \<L>\<^sub>a\<^sub>l\<^sub>l\<close>
+  assumes \<A>\<^sub>i\<^sub>n: \<open>literals_are_\<L>\<^sub>i\<^sub>n \<A> S\<close> and K: \<open>K \<in># \<L>\<^sub>a\<^sub>l\<^sub>l \<A>\<close>
   shows \<open>unit_propagation_inner_loop_wl_loop_D K S \<le>
-     \<Down> {((j', n', T'), j, n, T). j' = j \<and> n' = n \<and> T = T' \<and> literals_are_\<L>\<^sub>i\<^sub>n T'}
+     \<Down> {((j', n', T'), j, n, T). j' = j \<and> n' = n \<and> T = T' \<and> literals_are_\<L>\<^sub>i\<^sub>n \<A> T'}
        (unit_propagation_inner_loop_wl_loop K S)\<close>
 proof -
   have u: \<open>unit_propagation_inner_loop_body_wl_D K j w S \<le>
-         \<Down> {((j', n', T'), j, n, T). j' = j \<and> n' = n \<and> T = T' \<and> literals_are_\<L>\<^sub>i\<^sub>n T'}
+         \<Down> {((j', n', T'), j, n, T). j' = j \<and> n' = n \<and> T = T' \<and> literals_are_\<L>\<^sub>i\<^sub>n \<A> T'}
            (unit_propagation_inner_loop_body_wl K' j' w' S')\<close>
-  if \<open>K \<in># \<L>\<^sub>a\<^sub>l\<^sub>l\<close> and \<open>literals_are_\<L>\<^sub>i\<^sub>n S\<close> and
+  if \<open>K \<in># \<L>\<^sub>a\<^sub>l\<^sub>l \<A>\<close> and \<open>literals_are_\<L>\<^sub>i\<^sub>n \<A> S\<close> and
     \<open>S = S'\<close> \<open>K = K'\<close> \<open>w = w'\<close> \<open>j'=j\<close>
   for S S' and w w' and K K' and j' j
-    using unit_propagation_inner_loop_body_wl_D_spec[of K S j w] that by auto
+    using unit_propagation_inner_loop_body_wl_D_spec[of K \<A> S j w] that by auto
 
   show ?thesis
     unfolding unit_propagation_inner_loop_wl_loop_D_def unit_propagation_inner_loop_wl_loop_def
     apply (refine_vcg u)
     subgoal using assms by auto
     subgoal using assms by auto
-    subgoal using assms unfolding unit_propagation_inner_loop_wl_loop_D_inv_def by auto
+    subgoal using assms unfolding unit_propagation_inner_loop_wl_loop_D_inv_def
+      by (auto dest: literals_are_\<L>\<^sub>i\<^sub>n_set_mset_\<L>\<^sub>a\<^sub>l\<^sub>l)
     subgoal by auto
     subgoal using K by auto
+    subgoal by auto
     subgoal by auto
     subgoal by auto
     subgoal by auto
@@ -947,28 +950,28 @@ proof -
     done
 qed
 
-definition (in isasat_input_ops) unit_propagation_inner_loop_wl_D
+definition unit_propagation_inner_loop_wl_D
  :: \<open>nat literal \<Rightarrow> nat twl_st_wl \<Rightarrow> nat twl_st_wl nres\<close> where
   \<open>unit_propagation_inner_loop_wl_D L S\<^sub>0 = do {
      (j, w, S) \<leftarrow> unit_propagation_inner_loop_wl_loop_D L S\<^sub>0;
-     ASSERT (j \<le> w \<and> w \<le> length (watched_by S L) \<and> L \<in># \<L>\<^sub>a\<^sub>l\<^sub>l);
+     ASSERT (j \<le> w \<and> w \<le> length (watched_by S L) \<and> L \<in># \<L>\<^sub>a\<^sub>l\<^sub>l (all_atms_st S\<^sub>0));
      S \<leftarrow> cut_watch_list j w L S;
      RETURN S
   }\<close>
 
 lemma unit_propagation_inner_loop_wl_D_spec:
-  assumes \<A>\<^sub>i\<^sub>n: \<open>literals_are_\<L>\<^sub>i\<^sub>n S\<close> and K: \<open>K \<in># \<L>\<^sub>a\<^sub>l\<^sub>l\<close>
+  assumes \<A>\<^sub>i\<^sub>n: \<open>literals_are_\<L>\<^sub>i\<^sub>n \<A> S\<close> and K: \<open>K \<in># \<L>\<^sub>a\<^sub>l\<^sub>l \<A>\<close>
   shows \<open>unit_propagation_inner_loop_wl_D K S \<le>
-     \<Down> {(T', T). T = T' \<and> literals_are_\<L>\<^sub>i\<^sub>n T}
+     \<Down> {(T', T). T = T' \<and> literals_are_\<L>\<^sub>i\<^sub>n \<A> T}
        (unit_propagation_inner_loop_wl K S)\<close>
 proof -
   have cut_watch_list: \<open>cut_watch_list x1b x1c K x2c \<bind> RETURN
-        \<le> \<Down> {(T', T). T = T' \<and> literals_are_\<L>\<^sub>i\<^sub>n T}
+        \<le> \<Down> {(T', T). T = T' \<and> literals_are_\<L>\<^sub>i\<^sub>n \<A> T}
           (cut_watch_list x1 x1a K x2a)\<close>
     if
       \<open>(x, x')
       \<in> {((j', n', T'), j, n, T).
-          j' = j \<and> n' = n \<and> T = T' \<and> literals_are_\<L>\<^sub>i\<^sub>n T'}\<close> and
+          j' = j \<and> n' = n \<and> T = T' \<and> literals_are_\<L>\<^sub>i\<^sub>n \<A> T'}\<close> and
       \<open>x2 = (x1a, x2a)\<close> and
       \<open>x' = (x1, x2)\<close> and
       \<open>x2b = (x1c, x2c)\<close> and
@@ -977,29 +980,29 @@ proof -
     for x x' x1 x2 x1a x2a x1b x2b x1c x2c
   proof -
     show ?thesis
-      using that
-      by (cases x2c) (auto simp: cut_watch_list_def literals_are_\<L>\<^sub>i\<^sub>n_def
+      using that unfolding literals_are_\<L>\<^sub>i\<^sub>n_def
+      by (cases x2c) (auto simp: cut_watch_list_def
           blits_in_\<L>\<^sub>i\<^sub>n_def dest!: in_set_takeD in_set_dropD)
   qed
 
   show ?thesis
     unfolding unit_propagation_inner_loop_wl_D_def unit_propagation_inner_loop_wl_def
-    apply (refine_vcg unit_propagation_inner_loop_wl_spec)
+    apply (refine_vcg unit_propagation_inner_loop_wl_spec[of \<A>])
     subgoal using \<A>\<^sub>i\<^sub>n .
     subgoal using K .
     subgoal by auto
     subgoal by auto
-    subgoal using K by auto
+    subgoal using \<A>\<^sub>i\<^sub>n K by auto
     subgoal by (rule cut_watch_list)
     done
 qed
 
-definition (in isasat_input_ops)  unit_propagation_outer_loop_wl_D_inv where
+definition unit_propagation_outer_loop_wl_D_inv where
 \<open>unit_propagation_outer_loop_wl_D_inv S \<longleftrightarrow>
     unit_propagation_outer_loop_wl_inv S \<and>
-    literals_are_\<L>\<^sub>i\<^sub>n S\<close>
-
-definition (in isasat_input_ops) unit_propagation_outer_loop_wl_D
+    literals_are_\<L>\<^sub>i\<^sub>n (all_atms_st S) S\<close>
+      
+definition unit_propagation_outer_loop_wl_D
    :: \<open>nat twl_st_wl \<Rightarrow> nat twl_st_wl nres\<close>
 where
   \<open>unit_propagation_outer_loop_wl_D S\<^sub>0 =
@@ -1008,22 +1011,25 @@ where
       (\<lambda>S. do {
         ASSERT(literals_to_update_wl S \<noteq> {#});
         (S', L) \<leftarrow> select_and_remove_from_literals_to_update_wl S;
-        ASSERT(L \<in># all_lits_of_mm (mset `# ran_mf (get_clauses_wl S') +
-                        get_unit_clauses_wl S'));
+        ASSERT(L \<in># \<L>\<^sub>a\<^sub>l\<^sub>l (all_atms_st S));
         unit_propagation_inner_loop_wl_D L S'
       })
       (S\<^sub>0 :: nat twl_st_wl)\<close>
 
 lemma literals_are_\<L>\<^sub>i\<^sub>n_set_lits_to_upd[twl_st_wl, simp]:
-   \<open>literals_are_\<L>\<^sub>i\<^sub>n (set_literals_to_update_wl C S) \<longleftrightarrow> literals_are_\<L>\<^sub>i\<^sub>n S\<close>
+   \<open>literals_are_\<L>\<^sub>i\<^sub>n \<A> (set_literals_to_update_wl C S) \<longleftrightarrow> literals_are_\<L>\<^sub>i\<^sub>n \<A> S\<close>
   by (cases S) (auto simp: literals_are_\<L>\<^sub>i\<^sub>n_def blits_in_\<L>\<^sub>i\<^sub>n_def)
 
 lemma unit_propagation_outer_loop_wl_D_spec:
-  assumes \<A>\<^sub>i\<^sub>n: \<open>literals_are_\<L>\<^sub>i\<^sub>n S\<close>
+  assumes \<A>\<^sub>i\<^sub>n: \<open>literals_are_\<L>\<^sub>i\<^sub>n \<A> S\<close>
   shows \<open>unit_propagation_outer_loop_wl_D S \<le>
-     \<Down> {(T', T). T = T' \<and> literals_are_\<L>\<^sub>i\<^sub>n T}
+     \<Down> {(T', T). T = T' \<and> literals_are_\<L>\<^sub>i\<^sub>n \<A> T}
        (unit_propagation_outer_loop_wl S)\<close>
 proof -
+  have H: \<open>set_mset (all_lits_of_mm (mset `# ran_mf (get_clauses_wl S') + get_unit_clauses_wl S')) =
+    set_mset (\<L>\<^sub>a\<^sub>l\<^sub>l (all_atms_st S'))\<close> for S'
+    by (auto simp: in_all_lits_of_mm_ain_atms_of_iff all_atms_def all_lits_def
+      in_\<L>\<^sub>a\<^sub>l\<^sub>l_atm_of_\<A>\<^sub>i\<^sub>n)
   have select: \<open>select_and_remove_from_literals_to_update_wl S \<le>
     \<Down> {((T', L'), (T, L)). T = T' \<and> L = L' \<and>
         T = set_literals_to_update_wl (literals_to_update_wl S - {#L#}) S}
@@ -1032,46 +1038,45 @@ proof -
     unfolding select_and_remove_from_literals_to_update_wl_def select_and_remove_from_literals_to_update_def
     apply (rule RES_refine)
     using that unfolding select_and_remove_from_literals_to_update_wl_def by blast
-  have unit_prop: \<open>literals_are_\<L>\<^sub>i\<^sub>n S \<Longrightarrow>
-          K \<in># \<L>\<^sub>a\<^sub>l\<^sub>l \<Longrightarrow>
+  have unit_prop: \<open>literals_are_\<L>\<^sub>i\<^sub>n \<A> S \<Longrightarrow>
+          K \<in># \<L>\<^sub>a\<^sub>l\<^sub>l \<A> \<Longrightarrow>
           unit_propagation_inner_loop_wl_D K S
-          \<le> \<Down> {(T', T). T = T' \<and> literals_are_\<L>\<^sub>i\<^sub>n T} (unit_propagation_inner_loop_wl K' S')\<close>
+          \<le> \<Down> {(T', T). T = T' \<and> literals_are_\<L>\<^sub>i\<^sub>n \<A> T} (unit_propagation_inner_loop_wl K' S')\<close>
     if \<open>K = K'\<close> and \<open>S = S'\<close> for K K' and S S' :: \<open>nat twl_st_wl\<close>
     unfolding that by (rule unit_propagation_inner_loop_wl_D_spec)
   show ?thesis
-    unfolding unit_propagation_outer_loop_wl_D_def unit_propagation_outer_loop_wl_def
+    unfolding unit_propagation_outer_loop_wl_D_def unit_propagation_outer_loop_wl_def H
     apply (refine_vcg select unit_prop)
     subgoal using \<A>\<^sub>i\<^sub>n by simp
     subgoal unfolding unit_propagation_outer_loop_wl_D_inv_def by auto
     subgoal by auto
     subgoal by auto
-    subgoal by auto
+    subgoal using \<A>\<^sub>i\<^sub>n apply simp by auto
     subgoal by auto
     subgoal by auto
     subgoal using \<A>\<^sub>i\<^sub>n by (auto simp: twl_st_wl)
     subgoal for S' S T'L' TL T' L' T L
-      by auto
-        (auto simp add: is_\<L>\<^sub>a\<^sub>l\<^sub>l_def all_lits_of_mm_union
-          literals_are_\<L>\<^sub>i\<^sub>n_def)
+      using \<A>\<^sub>i\<^sub>n by auto
     done
 qed
 
 lemma unit_propagation_outer_loop_wl_D_spec':
-  shows \<open>(unit_propagation_outer_loop_wl_D, unit_propagation_outer_loop_wl) \<in> {(T', T). T = T' \<and> literals_are_\<L>\<^sub>i\<^sub>n T} \<rightarrow>\<^sub>f
-     \<langle>{(T', T). T = T' \<and> literals_are_\<L>\<^sub>i\<^sub>n T}\<rangle>nres_rel\<close>
+  shows \<open>(unit_propagation_outer_loop_wl_D, unit_propagation_outer_loop_wl) \<in>
+    {(T', T). T = T' \<and> literals_are_\<L>\<^sub>i\<^sub>n \<A> T} \<rightarrow>\<^sub>f
+     \<langle>{(T', T). T = T' \<and> literals_are_\<L>\<^sub>i\<^sub>n \<A> T}\<rangle>nres_rel\<close>
   apply (intro frefI nres_relI)
   subgoal for x y
     apply (rule order_trans)
-    apply (rule unit_propagation_outer_loop_wl_D_spec[of x])
+    apply (rule unit_propagation_outer_loop_wl_D_spec[of \<A> x])
      apply (auto simp: prod_rel_def intro: conc_fun_R_mono)
     done
   done
 
-definition (in isasat_input_ops) skip_and_resolve_loop_wl_D_inv where
+definition skip_and_resolve_loop_wl_D_inv where
   \<open>skip_and_resolve_loop_wl_D_inv S\<^sub>0 brk S \<equiv>
-      skip_and_resolve_loop_wl_inv S\<^sub>0 brk S \<and> literals_are_\<L>\<^sub>i\<^sub>n S\<close>
+      skip_and_resolve_loop_wl_inv S\<^sub>0 brk S \<and> literals_are_\<L>\<^sub>i\<^sub>n (all_atms_st S) S\<close>
 
-definition (in isasat_input_ops) skip_and_resolve_loop_wl_D
+definition skip_and_resolve_loop_wl_D
   :: \<open>nat twl_st_wl \<Rightarrow> nat twl_st_wl nres\<close>
 where
   \<open>skip_and_resolve_loop_wl_D S\<^sub>0 =
@@ -1101,18 +1106,29 @@ where
     }
   \<close>
 
-lemma (in isasat_input_ops) literals_are_\<L>\<^sub>i\<^sub>n_tl_state_wl[simp]:
-  \<open>literals_are_\<L>\<^sub>i\<^sub>n (tl_state_wl S) = literals_are_\<L>\<^sub>i\<^sub>n S\<close>
+lemma literals_are_\<L>\<^sub>i\<^sub>n_tl_state_wl[simp]:
+  \<open>literals_are_\<L>\<^sub>i\<^sub>n \<A> (tl_state_wl S) = literals_are_\<L>\<^sub>i\<^sub>n \<A> S\<close>
   by (cases S)
    (auto simp: is_\<L>\<^sub>a\<^sub>l\<^sub>l_def tl_state_wl_def literals_are_\<L>\<^sub>i\<^sub>n_def blits_in_\<L>\<^sub>i\<^sub>n_def)
 
 lemma get_clauses_wl_tl_state: \<open>get_clauses_wl (tl_state_wl T) = get_clauses_wl T\<close>
   unfolding tl_state_wl_def by (cases T) auto
 
+lemma blits_in_\<L>\<^sub>i\<^sub>n_skip_and_resolve[simp]:
+  \<open>blits_in_\<L>\<^sub>i\<^sub>n (tl x1aa, N, D, ar, as, at, bd) = blits_in_\<L>\<^sub>i\<^sub>n (x1aa, N, D, ar, as, at, bd)\<close>
+  \<open>blits_in_\<L>\<^sub>i\<^sub>n
+        (x1aa, N,
+         Some (resolve_cls_wl' (x1aa', N', x1ca', ar', as', at', bd') x2b
+            x1b),
+         ar, as, at, bd) =
+  blits_in_\<L>\<^sub>i\<^sub>n (x1aa, N, x1ca', ar, as, at, bd)\<close>
+  by (auto simp: blits_in_\<L>\<^sub>i\<^sub>n_def)
+
+
 lemma skip_and_resolve_loop_wl_D_spec:
-  assumes \<A>\<^sub>i\<^sub>n: \<open>literals_are_\<L>\<^sub>i\<^sub>n S\<close>
+  assumes \<A>\<^sub>i\<^sub>n: \<open>literals_are_\<L>\<^sub>i\<^sub>n \<A> S\<close>
   shows \<open>skip_and_resolve_loop_wl_D S \<le>
-     \<Down> {(T', T). T = T' \<and> literals_are_\<L>\<^sub>i\<^sub>n T \<and> get_clauses_wl T = get_clauses_wl S}
+     \<Down> {(T', T). T = T' \<and> literals_are_\<L>\<^sub>i\<^sub>n \<A> T \<and> get_clauses_wl T = get_clauses_wl S}
        (skip_and_resolve_loop_wl S)\<close>
     (is \<open>_ \<le> \<Down> ?R _\<close>)
 proof -
@@ -1120,7 +1136,6 @@ proof -
    \<open>invar = (\<lambda>(brk, T). skip_and_resolve_loop_wl_D_inv S brk T)\<close>
   have 1: \<open>((get_conflict_wl S = Some {#}, S), get_conflict_wl S = Some {#}, S) \<in> Id\<close>
     by auto
-
 
   show ?thesis
     unfolding skip_and_resolve_loop_wl_D_def skip_and_resolve_loop_wl_def
@@ -1138,7 +1153,7 @@ proof -
     subgoal by auto
     subgoal
       unfolding skip_and_resolve_loop_wl_D_inv_def update_confl_tl_wl_def
-      by (auto split: prod.splits simp: literals_are_\<L>\<^sub>i\<^sub>n_def blits_in_\<L>\<^sub>i\<^sub>n_def)
+      by (auto split: prod.splits simp: literals_are_\<L>\<^sub>i\<^sub>n_def)
     subgoal by auto
     subgoal by auto
     done
@@ -1155,13 +1170,13 @@ where
   \<open>list_of_mset2 L L' D =
     SPEC (\<lambda>E. mset E = D \<and> E!0 = L \<and> E!1 = L' \<and> length E \<ge> 2)\<close>
 
-definition (in -) single_of_mset where
+definition single_of_mset where
   \<open>single_of_mset D = SPEC(\<lambda>L. D = mset [L])\<close>
 
-definition (in isasat_input_ops) backtrack_wl_D_inv where
-  \<open>backtrack_wl_D_inv S \<longleftrightarrow> backtrack_wl_inv S \<and> literals_are_\<L>\<^sub>i\<^sub>n S\<close>
+definition backtrack_wl_D_inv where
+  \<open>backtrack_wl_D_inv S \<longleftrightarrow> backtrack_wl_inv S \<and> literals_are_\<L>\<^sub>i\<^sub>n (all_atms_st S) S\<close>
 
-definition (in isasat_input_ops) propagate_bt_wl_D
+definition propagate_bt_wl_D
   :: \<open>nat literal \<Rightarrow> nat literal \<Rightarrow> nat twl_st_wl \<Rightarrow> nat twl_st_wl nres\<close>
 where
   \<open>propagate_bt_wl_D = (\<lambda>L L' (M, N, D, NE, UE, Q, W). do {
@@ -1172,7 +1187,7 @@ where
           None, NE, UE, {#L#}, W(-L:= W (-L) @ [(i, L', b)], L':= W L' @ [(i, -L, b)]))
       })\<close>
 
-definition (in isasat_input_ops) propagate_unit_bt_wl_D
+definition propagate_unit_bt_wl_D
   :: \<open>nat literal \<Rightarrow> nat twl_st_wl \<Rightarrow> (nat twl_st_wl) nres\<close>
 where
   \<open>propagate_unit_bt_wl_D = (\<lambda>L (M, N, D, NE, UE, Q, W). do {
@@ -1180,7 +1195,7 @@ where
         RETURN (Propagated (-L) 0 # M, N, None, NE, add_mset {#D'#} UE, {#L#}, W)
     })\<close>
 
-definition (in isasat_input_ops) backtrack_wl_D :: \<open>nat twl_st_wl \<Rightarrow> nat twl_st_wl nres\<close> where
+definition backtrack_wl_D :: \<open>nat twl_st_wl \<Rightarrow> nat twl_st_wl nres\<close> where
   \<open>backtrack_wl_D S =
     do {
       ASSERT(backtrack_wl_D_inv S);
@@ -1200,16 +1215,17 @@ definition (in isasat_input_ops) backtrack_wl_D :: \<open>nat twl_st_wl \<Righta
 
 lemma backtrack_wl_D_spec:
   fixes S :: \<open>nat twl_st_wl\<close>
-  assumes \<A>\<^sub>i\<^sub>n: \<open>literals_are_\<L>\<^sub>i\<^sub>n S\<close> and confl: \<open>get_conflict_wl S ~= None\<close>
+  assumes \<A>\<^sub>i\<^sub>n: \<open>literals_are_\<L>\<^sub>i\<^sub>n \<A> S\<close> and confl: \<open>get_conflict_wl S \<noteq> None\<close>
   shows \<open>backtrack_wl_D S \<le>
-     \<Down> {(T', T). T = T' \<and> literals_are_\<L>\<^sub>i\<^sub>n T}
+     \<Down> {(T', T). T = T' \<and> literals_are_\<L>\<^sub>i\<^sub>n \<A> T}
        (backtrack_wl S)\<close>
 proof -
   have 1: \<open>((get_conflict_wl S = Some {#}, S), get_conflict_wl S = Some {#}, S) \<in> Id\<close>
     by auto
 
   have 3: \<open>find_lit_of_max_level_wl S M \<le>
-   \<Down> {(L', L). L' \<in># remove1_mset (-M) (the (get_conflict_wl S)) \<and> L' = L} (find_lit_of_max_level_wl S' M')\<close>
+     \<Down>{(L', L). L' \<in># remove1_mset (-M) (the (get_conflict_wl S)) \<and> L' = L}
+      (find_lit_of_max_level_wl S' M')\<close>
     if \<open>S = S'\<close> and \<open>M = M'\<close>
     for S S' :: \<open>nat twl_st_wl\<close> and M M'
     using that by (cases S; cases S') (auto simp: find_lit_of_max_level_wl_def intro!: RES_refine)
@@ -1285,11 +1301,11 @@ proof -
     using that unfolding find_lit_of_max_level_wl'_def find_lit_of_max_level_wl_def
     by (cases U) (auto 5 5 intro!: RES_refine)
 
-  have is_\<L>\<^sub>a\<^sub>l\<^sub>l_add: \<open>is_\<L>\<^sub>a\<^sub>l\<^sub>l (A + B) \<longleftrightarrow> set_mset A \<subseteq> set_mset \<L>\<^sub>a\<^sub>l\<^sub>l\<close> if \<open>is_\<L>\<^sub>a\<^sub>l\<^sub>l B\<close> for A B
+  have is_\<L>\<^sub>a\<^sub>l\<^sub>l_add: \<open>is_\<L>\<^sub>a\<^sub>l\<^sub>l \<A> (A + B) \<longleftrightarrow> set_mset A \<subseteq> set_mset (\<L>\<^sub>a\<^sub>l\<^sub>l \<A>)\<close> if \<open>is_\<L>\<^sub>a\<^sub>l\<^sub>l \<A> B\<close> for A B
     using that unfolding is_\<L>\<^sub>a\<^sub>l\<^sub>l_def by auto
 
   have propagate_bt_wl_D: \<open>propagate_bt_wl_D (lit_of (hd (get_trail_wl S))) L U
-        \<le> \<Down> {(T', T). T = T' \<and> literals_are_\<L>\<^sub>i\<^sub>n T}
+        \<le> \<Down> {(T', T). T = T' \<and> literals_are_\<L>\<^sub>i\<^sub>n \<A> T}
            (propagate_bt_wl (lit_of (hd (get_trail_wl S))) L' U')\<close>
     if
       \<open>backtrack_wl_inv S\<close> and
@@ -1371,7 +1387,7 @@ proof -
            ([- lit_of (hd (get_trail_wl S)), L'] @
             remove1 (- lit_of (hd (get_trail_wl S))) (remove1 L' D')) =
           2)]))
-    \<in> {(T', T). T = T' \<and> literals_are_\<L>\<^sub>i\<^sub>n T}\<close>
+    \<in> {(T', T). T = T' \<and> literals_are_\<L>\<^sub>i\<^sub>n \<A> T}\<close>
       if
         DD': \<open>(D, D') \<in> list_of_mset (the (Some DT)) (- lit_of (hd (get_trail_wl S))) L\<close> and
         ii': \<open>(i, i') \<in> {(i, i'). i = i' \<and> i \<notin># dom_m NS}\<close>
@@ -1401,14 +1417,28 @@ proof -
         apply (subst 1[symmetric])
         unfolding set_append list.sel
         by (rule list.set_intros)
+      have \<open>set_mset (all_lits_of_m (mset D)) \<subseteq>
+          set_mset (all_lits_of_mm ({#mset (fst x). x \<in># ran_m NS#} + (NES + UES)))\<close>
+	by (auto dest!: H[unfolded DT_D])
+      then have [simp]: \<open>is_\<L>\<^sub>a\<^sub>l\<^sub>l \<A> (all_lits (fmupd i' (D, False) NS) (NES + UES)) =
+          is_\<L>\<^sub>a\<^sub>l\<^sub>l \<A> (all_lits NS (NES + UES))\<close>
+	\<open>set_mset (\<L>\<^sub>a\<^sub>l\<^sub>l (atm_of `# all_lits (fmupd i' (D, False) NS) (NES + UES))) =
+ 	  set_mset (\<L>\<^sub>a\<^sub>l\<^sub>l (atm_of `# all_lits NS (NES + UES)))\<close>	
+	using i'_dom unfolding is_\<L>\<^sub>a\<^sub>l\<^sub>l_def all_lits_def
+	by (auto 5 5 simp add: ran_m_mapsto_upd_notin all_lits_of_mm_add_mset
+	  in_\<L>\<^sub>a\<^sub>l\<^sub>l_atm_of_\<A>\<^sub>i\<^sub>n atm_of_eq_atm_of)
+
       have \<open>x \<in># all_lits_of_mm ({#mset (fst x). x \<in># ran_m NS#} + (NES + UES)) \<Longrightarrow>
-        x \<in># \<L>\<^sub>a\<^sub>l\<^sub>l\<close> for x
-        using i'_dom \<A>\<^sub>i\<^sub>n is_\<L>\<^sub>a\<^sub>l\<^sub>l_def by (fastforce simp: S literals_are_\<L>\<^sub>i\<^sub>n_def)
+        x \<in># \<L>\<^sub>a\<^sub>l\<^sub>l \<A>\<close> for x
+        using i'_dom \<A>\<^sub>i\<^sub>n unfolding is_\<L>\<^sub>a\<^sub>l\<^sub>l_def literals_are_\<L>\<^sub>i\<^sub>n_def
+	by (auto simp: S all_lits_def)
       then show ?thesis
         using i'_dom \<A>\<^sub>i\<^sub>n K[OF \<open>L \<in> set D\<close>] K[OF \<open>- lit_of (hd MS) \<in> set D\<close>]
-        by (auto simp: ran_m_mapsto_upd_notin all_lits_of_mm_add_mset literals_are_\<L>\<^sub>i\<^sub>n_def
+	unfolding literals_are_\<L>\<^sub>i\<^sub>n_def
+        by (auto simp: ran_m_mapsto_upd_notin all_lits_of_mm_add_mset
             blits_in_\<L>\<^sub>i\<^sub>n_def is_\<L>\<^sub>a\<^sub>l\<^sub>l_add S dest!: H[unfolded DT_D])
     qed
+
     define get_fresh_index2 where
       \<open>get_fresh_index2 N NUE W = get_fresh_index_wl (N :: nat clauses_l) (NUE :: nat clauses)
           (W::nat literal \<Rightarrow> (nat watcher) list)\<close>
@@ -1436,7 +1466,7 @@ proof -
 
   have propagate_unit_bt_wl_D: \<open>propagate_unit_bt_wl_D (lit_of (hd (get_trail_wl S))) U
     \<le> SPEC (\<lambda>c. (c, propagate_unit_bt_wl (lit_of (hd (get_trail_wl S))) U')
-                 \<in> {(T', T). T = T' \<and> literals_are_\<L>\<^sub>i\<^sub>n T})\<close>
+                 \<in> {(T', T). T = T' \<and> literals_are_\<L>\<^sub>i\<^sub>n \<A> T})\<close>
     if
       \<open>backtrack_wl_inv S\<close> and
       bt: \<open>backtrack_wl_D_inv S\<close> and
@@ -1490,18 +1520,28 @@ proof -
         x \<in># all_lits_of_mm ({#mset x. x \<in># ran_mf NS#} + NES)\<close>
       for x
       using DT all_lits_of_m_mono by blast
-    then have \<A>\<^sub>i\<^sub>n_D: \<open>literals_are_in_\<L>\<^sub>i\<^sub>n DT\<close>
+    then have \<A>\<^sub>i\<^sub>n_D: \<open>literals_are_in_\<L>\<^sub>i\<^sub>n \<A> DT\<close>
       using DT \<A>\<^sub>i\<^sub>n unfolding literals_are_in_\<L>\<^sub>i\<^sub>n_def S is_\<L>\<^sub>a\<^sub>l\<^sub>l_def literals_are_\<L>\<^sub>i\<^sub>n_def
-      by (auto simp: all_lits_of_mm_union)
+      by (auto simp: all_lits_of_mm_union all_lits_def)
+    have [simp]: \<open>is_\<L>\<^sub>a\<^sub>l\<^sub>l \<A> (all_lits NS (add_mset {#x#} (NES + UES))) =
+      is_\<L>\<^sub>a\<^sub>l\<^sub>l \<A> (all_lits NS (NES + UES))\<close>
+      \<open>set_mset (\<L>\<^sub>a\<^sub>l\<^sub>l (atm_of `# all_lits NS (add_mset {#x#} (NES + UES)))) =
+       set_mset (\<L>\<^sub>a\<^sub>l\<^sub>l (atm_of `# all_lits NS (NES + UES)))\<close>
+      if \<open>DT = {#x#}\<close>
+      for x
+      using H[of x] H[of \<open>-x\<close>] that
+      unfolding is_\<L>\<^sub>a\<^sub>l\<^sub>l_def all_lits_def
+      by (auto simp add: all_lits_of_mm_add_mset in_\<L>\<^sub>a\<^sub>l\<^sub>l_atm_of_\<A>\<^sub>i\<^sub>n atm_of_eq_atm_of
+        all_lits_of_m_add_mset insert_absorb all_lits_of_mm_union)
 
     show ?thesis
       unfolding propagate_unit_bt_wl_D_def propagate_unit_bt_wl_def U U' single_of_mset_def
       apply clarify
       apply refine_vcg
-      using \<A>\<^sub>i\<^sub>n_D \<A>\<^sub>i\<^sub>n
+      using \<A>\<^sub>i\<^sub>n_D \<A>\<^sub>i\<^sub>n unfolding literals_are_\<L>\<^sub>i\<^sub>n_def
       by (auto simp: clauses_def mset_take_mset_drop_mset mset_take_mset_drop_mset'
           all_lits_of_mm_add_mset is_\<L>\<^sub>a\<^sub>l\<^sub>l_add literals_are_in_\<L>\<^sub>i\<^sub>n_def S
-          literals_are_\<L>\<^sub>i\<^sub>n_def blits_in_\<L>\<^sub>i\<^sub>n_def)
+          blits_in_\<L>\<^sub>i\<^sub>n_def)
   qed
   show ?thesis
     unfolding backtrack_wl_D_def backtrack_wl_def find_lit_of_max_level_wl'_def
@@ -1518,26 +1558,26 @@ qed
 
 
 subsubsection \<open>Decide or Skip\<close>
-thm find_unassigned_lit_wl_def
-definition (in isasat_input_ops) find_unassigned_lit_wl_D
+
+definition find_unassigned_lit_wl_D
   :: \<open>nat twl_st_wl \<Rightarrow> (nat twl_st_wl \<times> nat literal option) nres\<close>
 where
   \<open>find_unassigned_lit_wl_D S = (
      SPEC(\<lambda>((M, N, D, NE, UE, WS, Q), L).
          S = (M, N, D, NE, UE, WS, Q) \<and>
          (L \<noteq> None \<longrightarrow>
-            undefined_lit M (the L) \<and> the L \<in># \<L>\<^sub>a\<^sub>l\<^sub>l \<and>
+            undefined_lit M (the L) \<and> the L \<in># \<L>\<^sub>a\<^sub>l\<^sub>l (all_atms N NE) \<and>
             atm_of (the L) \<in> atms_of_mm (clause `# twl_clause_of `# init_clss_lf N + NE)) \<and>
          (L = None \<longrightarrow> (\<nexists>L'. undefined_lit M L' \<and>
             atm_of L' \<in> atms_of_mm (clause `# twl_clause_of `# init_clss_lf N + NE)))))
 \<close>
 
 
-definition (in isasat_input_ops) decide_wl_or_skip_D_pre :: \<open>nat twl_st_wl \<Rightarrow> bool\<close> where
+definition decide_wl_or_skip_D_pre :: \<open>nat twl_st_wl \<Rightarrow> bool\<close> where
 \<open>decide_wl_or_skip_D_pre S \<longleftrightarrow>
-   decide_wl_or_skip_pre S \<and> literals_are_\<L>\<^sub>i\<^sub>n S\<close>
+   decide_wl_or_skip_pre S \<and> literals_are_\<L>\<^sub>i\<^sub>n (all_atms_st S) S\<close>
 
-definition(in isasat_input_ops)  decide_wl_or_skip_D
+definition decide_wl_or_skip_D
   :: \<open>nat twl_st_wl \<Rightarrow> (bool \<times> nat twl_st_wl) nres\<close>
 where
   \<open>decide_wl_or_skip_D S = (do {
@@ -1550,11 +1590,11 @@ where
 \<close>
 
 theorem decide_wl_or_skip_D_spec:
-  assumes \<open>literals_are_\<L>\<^sub>i\<^sub>n S\<close>
+  assumes \<open>literals_are_\<L>\<^sub>i\<^sub>n \<A> S\<close>
   shows \<open>decide_wl_or_skip_D S
-    \<le> \<Down> {((b', T'), b, T). b = b' \<and> T = T' \<and> literals_are_\<L>\<^sub>i\<^sub>n T} (decide_wl_or_skip S)\<close>
+    \<le> \<Down> {((b', T'), b, T). b = b' \<and> T = T' \<and> literals_are_\<L>\<^sub>i\<^sub>n \<A> T} (decide_wl_or_skip S)\<close>
 proof -
-  have H: \<open>find_unassigned_lit_wl_D S \<le> \<Down> {((S', L'), L). S' = S \<and> L = L' \<and>
+  have H: \<open>find_unassigned_lit_wl_D S \<le> \<Down> {((S', L'), L). S' = S \<and> L = L' \<and> literals_are_\<L>\<^sub>i\<^sub>n \<A> S \<and>
          (L \<noteq> None \<longrightarrow>
             undefined_lit (get_trail_wl S) (the L) \<and>
             atm_of (the L) \<in> atms_of_mm (clause `# twl_clause_of `# init_clss_lf (get_clauses_wl S)
@@ -1564,17 +1604,17 @@ proof -
                  + get_unit_init_clss_wl S)))}
      (find_unassigned_lit_wl S')\<close>
     (is \<open>_ \<le> \<Down> ?find _\<close>)
-    if \<open>S = S'\<close>
+    if \<open>S = S'\<close> and \<open>literals_are_\<L>\<^sub>i\<^sub>n \<A> S\<close>
     for S S' :: \<open>nat twl_st_wl\<close>
-    unfolding find_unassigned_lit_wl_def find_unassigned_lit_wl_D_def that
+    using that(2) unfolding find_unassigned_lit_wl_def find_unassigned_lit_wl_D_def that(1)
     by (cases S') (auto intro!: RES_refine simp: mset_take_mset_drop_mset')
   have [refine]: \<open>x = x' \<Longrightarrow> (x, x') \<in> \<langle>Id\<rangle> option_rel\<close>
     for x x' by auto
   have decide_lit_wl: \<open>((False, decide_lit_wl L T), False, decide_lit_wl L' S')
         \<in> {((b', T'), b, T).
-            b = b' \<and> T = T' \<and> literals_are_\<L>\<^sub>i\<^sub>n T}\<close>
+            b = b' \<and> T = T' \<and> literals_are_\<L>\<^sub>i\<^sub>n \<A> T}\<close>
     if
-      SS': \<open>(S, S') \<in> {(T', T). T = T' \<and> literals_are_\<L>\<^sub>i\<^sub>n T}\<close> and
+      SS': \<open>(S, S') \<in> {(T', T). T = T' \<and> literals_are_\<L>\<^sub>i\<^sub>n \<A> T}\<close> and
       \<open>decide_wl_or_skip_pre S'\<close> and
       pre: \<open>decide_wl_or_skip_D_pre S\<close> and
       LT_L': \<open>(LT, bL') \<in> ?find S\<close> and
@@ -1584,11 +1624,12 @@ proof -
       LL': \<open>(L, L') \<in> Id\<close>
     for S S' L L' LT bL bL' T
   proof -
-    have \<A>\<^sub>i\<^sub>n: \<open>literals_are_\<L>\<^sub>i\<^sub>n T\<close> and [simp]: \<open>T = S\<close>
-      using LT_L' pre unfolding LT decide_wl_or_skip_D_pre_def by fast+
+    have \<A>\<^sub>i\<^sub>n: \<open>literals_are_\<L>\<^sub>i\<^sub>n \<A> T\<close> and [simp]: \<open>T = S\<close>
+      using LT_L' pre unfolding LT decide_wl_or_skip_D_pre_def 
+   by fast+
     have [simp]: \<open>S' = S\<close> \<open>L = L'\<close>
       using SS' LL' by simp_all
-    have \<open>literals_are_\<L>\<^sub>i\<^sub>n (decide_lit_wl L' S)\<close>
+    have \<open>literals_are_\<L>\<^sub>i\<^sub>n \<A> (decide_lit_wl L' S)\<close>
       using \<A>\<^sub>i\<^sub>n
       by (cases S) (auto simp: decide_lit_wl_def clauses_def blits_in_\<L>\<^sub>i\<^sub>n_def
           literals_are_\<L>\<^sub>i\<^sub>n_def)
@@ -1596,13 +1637,14 @@ proof -
       by auto
   qed
 
-  have \<open>(decide_wl_or_skip_D, decide_wl_or_skip) \<in> {((T'), (T)).  T = T' \<and> literals_are_\<L>\<^sub>i\<^sub>n T} \<rightarrow>\<^sub>f
-     \<langle>{((b', T'), (b, T)). b = b' \<and> T = T' \<and> literals_are_\<L>\<^sub>i\<^sub>n T}\<rangle> nres_rel\<close>
+  have \<open>(decide_wl_or_skip_D, decide_wl_or_skip) \<in> {(T', T).  T = T' \<and> literals_are_\<L>\<^sub>i\<^sub>n \<A> T} \<rightarrow>\<^sub>f
+     \<langle>{((b', T'), (b, T)). b = b' \<and> T = T' \<and> literals_are_\<L>\<^sub>i\<^sub>n \<A> T}\<rangle> nres_rel\<close>
     unfolding decide_wl_or_skip_D_def decide_wl_or_skip_def
     apply (intro frefI)
     apply (refine_vcg H)
     subgoal unfolding decide_wl_or_skip_D_pre_def by blast
     subgoal by simp
+    subgoal by auto
     subgoal by simp
     subgoal unfolding decide_wl_or_skip_D_pre_def by fast
     subgoal by (rule decide_lit_wl) assumption+
@@ -1611,12 +1653,13 @@ proof -
     using assms by (cases S) (auto simp: fref_def nres_rel_def)
 qed
 
+
 subsubsection \<open>Backtrack, Skip, Resolve or Decide\<close>
 
-definition (in isasat_input_ops) cdcl_twl_o_prog_wl_D_pre where
-\<open>cdcl_twl_o_prog_wl_D_pre S \<longleftrightarrow> cdcl_twl_o_prog_wl_pre S \<and> literals_are_\<L>\<^sub>i\<^sub>n S\<close>
+definition cdcl_twl_o_prog_wl_D_pre where
+\<open>cdcl_twl_o_prog_wl_D_pre S \<longleftrightarrow> cdcl_twl_o_prog_wl_pre S \<and> literals_are_\<L>\<^sub>i\<^sub>n (all_atms_st S) S\<close>
 
-definition (in isasat_input_ops) cdcl_twl_o_prog_wl_D
+definition cdcl_twl_o_prog_wl_D
  :: \<open>nat twl_st_wl \<Rightarrow> (bool \<times> nat twl_st_wl) nres\<close>
 where
   \<open>cdcl_twl_o_prog_wl_D S =
@@ -1638,26 +1681,26 @@ where
   \<close>
 
 theorem cdcl_twl_o_prog_wl_D_spec:
-  assumes \<open>literals_are_\<L>\<^sub>i\<^sub>n S\<close>
-  shows \<open>cdcl_twl_o_prog_wl_D S \<le> \<Down> {((b', T'), (b, T)). b = b' \<and> T = T' \<and> literals_are_\<L>\<^sub>i\<^sub>n T}
+  assumes \<open>literals_are_\<L>\<^sub>i\<^sub>n \<A> S\<close>
+  shows \<open>cdcl_twl_o_prog_wl_D S \<le> \<Down> {((b', T'), (b, T)). b = b' \<and> T = T' \<and> literals_are_\<L>\<^sub>i\<^sub>n \<A> T}
      (cdcl_twl_o_prog_wl S)\<close>
 proof -
   have 1: \<open>backtrack_wl_D S \<le>
-     \<Down> {(T', T). T = T' \<and> literals_are_\<L>\<^sub>i\<^sub>n T}
-       (backtrack_wl T)\<close> if \<open>literals_are_\<L>\<^sub>i\<^sub>n S\<close> and \<open>get_conflict_wl S ~= None\<close> and \<open>S = T\<close>
+     \<Down> {(T', T). T = T' \<and> literals_are_\<L>\<^sub>i\<^sub>n \<A> T}
+       (backtrack_wl T)\<close> if \<open>literals_are_\<L>\<^sub>i\<^sub>n \<A> S\<close> and \<open>get_conflict_wl S \<noteq> None\<close> and \<open>S = T\<close>
     for S T
-    using backtrack_wl_D_spec[of S] that by fast
+    using backtrack_wl_D_spec[of \<A> S] that by fast
   have 2: \<open>skip_and_resolve_loop_wl_D S \<le>
-     \<Down> {(T', T). T = T' \<and> literals_are_\<L>\<^sub>i\<^sub>n T \<and>  get_clauses_wl T = get_clauses_wl S}
+     \<Down> {(T', T). T = T' \<and> literals_are_\<L>\<^sub>i\<^sub>n \<A> T \<and>  get_clauses_wl T = get_clauses_wl S}
         (skip_and_resolve_loop_wl T)\<close>
-    if \<A>\<^sub>i\<^sub>n: \<open>literals_are_\<L>\<^sub>i\<^sub>n S\<close> \<open>S = T\<close>
+    if \<A>\<^sub>i\<^sub>n: \<open>literals_are_\<L>\<^sub>i\<^sub>n \<A> S\<close> \<open>S = T\<close>
     for S T
-    using skip_and_resolve_loop_wl_D_spec[of S] that by fast
+    using skip_and_resolve_loop_wl_D_spec[of \<A> S] that by fast
   show ?thesis
     using assms
     unfolding cdcl_twl_o_prog_wl_D_def cdcl_twl_o_prog_wl_def
     apply (refine_vcg decide_wl_or_skip_D_spec 1 2)
-    subgoal unfolding cdcl_twl_o_prog_wl_D_pre_def by simp
+    subgoal unfolding cdcl_twl_o_prog_wl_D_pre_def by auto
     subgoal by simp
     subgoal by simp
     subgoal by simp
@@ -1672,14 +1715,13 @@ proof -
 qed
 
 theorem cdcl_twl_o_prog_wl_D_spec':
-  shows
   \<open>(cdcl_twl_o_prog_wl_D, cdcl_twl_o_prog_wl) \<in>
-    {(S,S'). (S,S') \<in> Id \<and>literals_are_\<L>\<^sub>i\<^sub>n S} \<rightarrow>\<^sub>f
-    \<langle>bool_rel \<times>\<^sub>r {(T', T). T = T' \<and> literals_are_\<L>\<^sub>i\<^sub>n T}\<rangle> nres_rel\<close>
+    {(S,S'). (S,S') \<in> Id \<and>literals_are_\<L>\<^sub>i\<^sub>n \<A> S} \<rightarrow>\<^sub>f
+    \<langle>bool_rel \<times>\<^sub>r {(T', T). T = T' \<and> literals_are_\<L>\<^sub>i\<^sub>n \<A> T}\<rangle> nres_rel\<close>
   apply (intro frefI nres_relI)
   subgoal for x y
     apply (rule order_trans)
-    apply (rule cdcl_twl_o_prog_wl_D_spec[of x])
+    apply (rule cdcl_twl_o_prog_wl_D_spec[of \<A> x])
      apply (auto simp: prod_rel_def intro: conc_fun_R_mono)
     done
   done
@@ -1687,14 +1729,14 @@ theorem cdcl_twl_o_prog_wl_D_spec':
 
 subsubsection \<open>Full Strategy\<close>
 
-definition (in isasat_input_ops) cdcl_twl_stgy_prog_wl_D
+definition cdcl_twl_stgy_prog_wl_D
    :: \<open>nat twl_st_wl \<Rightarrow> nat twl_st_wl nres\<close>
 where
   \<open>cdcl_twl_stgy_prog_wl_D S\<^sub>0 =
   do {
     do {
-      (brk, T) \<leftarrow> WHILE\<^sub>T\<^bsup>\<lambda>(brk, T). cdcl_twl_stgy_prog_wl_inv S\<^sub>0 (brk, T)\<and>
-          literals_are_\<L>\<^sub>i\<^sub>n T\<^esup>
+      (brk, T) \<leftarrow> WHILE\<^sub>T\<^bsup>\<lambda>(brk, T). cdcl_twl_stgy_prog_wl_inv S\<^sub>0 (brk, T) \<and>
+          literals_are_\<L>\<^sub>i\<^sub>n (all_atms_st T) T\<^esup>
         (\<lambda>(brk, _). \<not>brk)
         (\<lambda>(brk, S).
         do {
@@ -1708,18 +1750,19 @@ where
   \<close>
 
 theorem cdcl_twl_stgy_prog_wl_D_spec:
-  assumes \<open>literals_are_\<L>\<^sub>i\<^sub>n S\<close>
-  shows \<open>cdcl_twl_stgy_prog_wl_D S \<le> \<Down> {(T', T). T = T' \<and> literals_are_\<L>\<^sub>i\<^sub>n T}
+  assumes \<open>literals_are_\<L>\<^sub>i\<^sub>n \<A> S\<close>
+  shows \<open>cdcl_twl_stgy_prog_wl_D S \<le> \<Down> {(T', T). T = T' \<and> literals_are_\<L>\<^sub>i\<^sub>n \<A> T}
      (cdcl_twl_stgy_prog_wl S)\<close>
 proof -
-  have 1: \<open>((False, S), False, S) \<in> {((brk', T'), brk, T). brk = brk' \<and> T = T' \<and> literals_are_\<L>\<^sub>i\<^sub>n T}\<close>
+  have 1: \<open>((False, S), False, S) \<in> {((brk', T'), brk, T). brk = brk' \<and> T = T' \<and>
+      literals_are_\<L>\<^sub>i\<^sub>n \<A> T}\<close>
     using assms by fast
-  have 2: \<open>unit_propagation_outer_loop_wl_D S \<le> \<Down> {(T', T). T = T' \<and> literals_are_\<L>\<^sub>i\<^sub>n T}
-       (unit_propagation_outer_loop_wl T)\<close> if \<open>S = T\<close> \<open>literals_are_\<L>\<^sub>i\<^sub>n S\<close> for S T
-    using unit_propagation_outer_loop_wl_D_spec[of S] that by fast
-  have 3: \<open>cdcl_twl_o_prog_wl_D S \<le> \<Down> {((b', T'), b, T). b = b' \<and> T = T' \<and> literals_are_\<L>\<^sub>i\<^sub>n T}
-    (cdcl_twl_o_prog_wl T)\<close> if \<open>S = T\<close> \<open>literals_are_\<L>\<^sub>i\<^sub>n S\<close> for S T
-    using cdcl_twl_o_prog_wl_D_spec[of S] that by fast
+  have 2: \<open>unit_propagation_outer_loop_wl_D S \<le> \<Down> {(T', T). T = T' \<and> literals_are_\<L>\<^sub>i\<^sub>n \<A> T}
+       (unit_propagation_outer_loop_wl T)\<close> if \<open>S = T\<close> \<open>literals_are_\<L>\<^sub>i\<^sub>n \<A> S\<close> for S T
+    using unit_propagation_outer_loop_wl_D_spec[of \<A> S] that by fast
+  have 3: \<open>cdcl_twl_o_prog_wl_D S \<le> \<Down> {((b', T'), b, T). b = b' \<and> T = T' \<and> literals_are_\<L>\<^sub>i\<^sub>n \<A> T}
+    (cdcl_twl_o_prog_wl T)\<close> if \<open>S = T\<close> \<open>literals_are_\<L>\<^sub>i\<^sub>n \<A> S\<close> for S T
+    using cdcl_twl_o_prog_wl_D_spec[of \<A> S] that by fast
   show ?thesis
     unfolding cdcl_twl_stgy_prog_wl_D_def cdcl_twl_stgy_prog_wl_def
     apply (refine_vcg 1 2 3)
@@ -1736,14 +1779,14 @@ qed
 
 lemma cdcl_twl_stgy_prog_wl_D_spec':
   \<open>(cdcl_twl_stgy_prog_wl_D, cdcl_twl_stgy_prog_wl) \<in>
-    {(S,S'). (S,S') \<in> Id \<and>literals_are_\<L>\<^sub>i\<^sub>n S} \<rightarrow>\<^sub>f
-    \<langle>{(T', T). T = T' \<and> literals_are_\<L>\<^sub>i\<^sub>n T}\<rangle> nres_rel\<close>
+    {(S,S'). (S,S') \<in> Id \<and>literals_are_\<L>\<^sub>i\<^sub>n \<A> S} \<rightarrow>\<^sub>f
+    \<langle>{(T', T). T = T' \<and> literals_are_\<L>\<^sub>i\<^sub>n \<A> T}\<rangle> nres_rel\<close>
   by (intro frefI nres_relI)
     (auto intro: cdcl_twl_stgy_prog_wl_D_spec)
 
-definition (in isasat_input_ops) cdcl_twl_stgy_prog_wl_D_pre where
+definition cdcl_twl_stgy_prog_wl_D_pre where
   \<open>cdcl_twl_stgy_prog_wl_D_pre S U \<longleftrightarrow>
-    (cdcl_twl_stgy_prog_wl_pre S U \<and> literals_are_\<L>\<^sub>i\<^sub>n S)\<close>
+    (cdcl_twl_stgy_prog_wl_pre S U \<and> literals_are_\<L>\<^sub>i\<^sub>n (all_atms_st S) S)\<close>
 
 lemma cdcl_twl_stgy_prog_wl_D_spec_final:
   assumes
@@ -1751,10 +1794,10 @@ lemma cdcl_twl_stgy_prog_wl_D_spec_final:
   shows
     \<open>cdcl_twl_stgy_prog_wl_D S \<le> \<Down> (state_wl_l None O twl_st_l None) (conclusive_TWL_run S')\<close>
 proof -
-  have T: \<open>cdcl_twl_stgy_prog_wl_pre S S' \<and> literals_are_\<L>\<^sub>i\<^sub>n S\<close>
+  have T: \<open>cdcl_twl_stgy_prog_wl_pre S S' \<and> literals_are_\<L>\<^sub>i\<^sub>n (all_atms_st S) S\<close>
     using assms unfolding cdcl_twl_stgy_prog_wl_D_pre_def by blast
   show ?thesis
-    apply (rule order_trans[OF cdcl_twl_stgy_prog_wl_D_spec])
+    apply (rule order_trans[OF cdcl_twl_stgy_prog_wl_D_spec[of \<open>all_atms_st S\<close>]])
     subgoal using T by auto
     subgoal
       apply (rule order_trans)
@@ -1767,14 +1810,13 @@ proof -
 qed
 
 
-definition (in isasat_input_ops) cdcl_twl_stgy_prog_break_wl_D
-   :: \<open>nat twl_st_wl \<Rightarrow> nat twl_st_wl nres\<close>
+definition cdcl_twl_stgy_prog_break_wl_D :: \<open>nat twl_st_wl \<Rightarrow> nat twl_st_wl nres\<close>
 where
   \<open>cdcl_twl_stgy_prog_break_wl_D S\<^sub>0 =
   do {
     b \<leftarrow> SPEC (\<lambda>_. True);
     (b, brk, T) \<leftarrow> WHILE\<^sub>T\<^bsup>\<lambda>(b, brk, T). cdcl_twl_stgy_prog_wl_inv S\<^sub>0 (brk, T) \<and>
-          literals_are_\<L>\<^sub>i\<^sub>n T\<^esup>
+          literals_are_\<L>\<^sub>i\<^sub>n (all_atms_st T) T\<^esup>
         (\<lambda>(b, brk, _). b \<and> \<not>brk)
         (\<lambda>(b, brk, S).
         do {
@@ -1790,27 +1832,27 @@ where
   }\<close>
 
 theorem cdcl_twl_stgy_prog_break_wl_D_spec:
-  assumes \<open>literals_are_\<L>\<^sub>i\<^sub>n S\<close>
-  shows \<open>cdcl_twl_stgy_prog_break_wl_D S \<le> \<Down> {(T', T). T = T' \<and> literals_are_\<L>\<^sub>i\<^sub>n T}
+  assumes \<open>literals_are_\<L>\<^sub>i\<^sub>n \<A> S\<close>
+  shows \<open>cdcl_twl_stgy_prog_break_wl_D S \<le> \<Down> {(T', T). T = T' \<and> literals_are_\<L>\<^sub>i\<^sub>n \<A> T}
      (cdcl_twl_stgy_prog_break_wl S)\<close>
 proof -
   define f where \<open>f \<equiv> SPEC (\<lambda>_::bool. True)\<close>
   have 1: \<open>((b, False, S), b, False, S) \<in> {((b', brk', T'), b, brk, T). b = b' \<and> brk = brk' \<and>
-        T = T' \<and> literals_are_\<L>\<^sub>i\<^sub>n T}\<close>
+        T = T' \<and> literals_are_\<L>\<^sub>i\<^sub>n \<A> T}\<close>
     for b
     using assms by fast
   have 1: \<open>((b, False, S), b', False, S) \<in> {((b', brk', T'), b, brk, T). b = b' \<and> brk = brk' \<and>
-        T = T' \<and> literals_are_\<L>\<^sub>i\<^sub>n T}\<close>
+        T = T' \<and> literals_are_\<L>\<^sub>i\<^sub>n \<A> T}\<close>
     if \<open>(b, b') \<in> bool_rel\<close>
     for b b'
     using assms that by fast
 
-  have 2: \<open>unit_propagation_outer_loop_wl_D S \<le> \<Down> {(T', T). T = T' \<and> literals_are_\<L>\<^sub>i\<^sub>n T}
-       (unit_propagation_outer_loop_wl T)\<close> if \<open>S = T\<close> \<open>literals_are_\<L>\<^sub>i\<^sub>n S\<close> for S T
-    using unit_propagation_outer_loop_wl_D_spec[of S] that by fast
-  have 3: \<open>cdcl_twl_o_prog_wl_D S \<le> \<Down> {((b', T'), b, T). b = b' \<and> T = T' \<and> literals_are_\<L>\<^sub>i\<^sub>n T}
-    (cdcl_twl_o_prog_wl T)\<close> if \<open>S = T\<close> \<open>literals_are_\<L>\<^sub>i\<^sub>n S\<close> for S T
-    using cdcl_twl_o_prog_wl_D_spec[of S] that by fast
+  have 2: \<open>unit_propagation_outer_loop_wl_D S \<le> \<Down> {(T', T). T = T' \<and> literals_are_\<L>\<^sub>i\<^sub>n \<A> T}
+       (unit_propagation_outer_loop_wl T)\<close> if \<open>S = T\<close> \<open>literals_are_\<L>\<^sub>i\<^sub>n \<A> S\<close> for S T
+    using unit_propagation_outer_loop_wl_D_spec[of \<A> S] that by fast
+  have 3: \<open>cdcl_twl_o_prog_wl_D S \<le> \<Down> {((b', T'), b, T). b = b' \<and> T = T' \<and> literals_are_\<L>\<^sub>i\<^sub>n \<A> T}
+    (cdcl_twl_o_prog_wl T)\<close> if \<open>S = T\<close> \<open>literals_are_\<L>\<^sub>i\<^sub>n \<A> S\<close> for S T
+    using cdcl_twl_o_prog_wl_D_spec[of \<A> S] that by fast
   show ?thesis
     unfolding cdcl_twl_stgy_prog_break_wl_D_def cdcl_twl_stgy_prog_break_wl_def f_def[symmetric]
     apply (refine_vcg 1 2 3)
@@ -1835,10 +1877,10 @@ lemma cdcl_twl_stgy_prog_break_wl_D_spec_final:
   shows
     \<open>cdcl_twl_stgy_prog_break_wl_D S \<le> \<Down> (state_wl_l None O twl_st_l None) (conclusive_TWL_run S')\<close>
 proof -
-  have T: \<open>cdcl_twl_stgy_prog_wl_pre S S' \<and> literals_are_\<L>\<^sub>i\<^sub>n S\<close>
+  have T: \<open>cdcl_twl_stgy_prog_wl_pre S S' \<and> literals_are_\<L>\<^sub>i\<^sub>n (all_atms_st S) S\<close>
     using assms unfolding cdcl_twl_stgy_prog_wl_D_pre_def by blast
   show ?thesis
-    apply (rule order_trans[OF cdcl_twl_stgy_prog_break_wl_D_spec])
+    apply (rule order_trans[OF cdcl_twl_stgy_prog_break_wl_D_spec[of \<open>all_atms_st S\<close>]])
     subgoal using T by auto
     subgoal
       apply (rule order_trans)
@@ -1849,8 +1891,6 @@ proof -
       done
     done
 qed
-
-end \<comment> \<open>end of locale @{locale isasat_input_ops}\<close>
 
 text \<open>The definition is here to be shared later.\<close>
 definition get_propagation_reason :: \<open>('v, 'mark) ann_lits \<Rightarrow> 'v literal \<Rightarrow> 'mark option nres\<close> where
